code/helperLib/thingsToSearch.v
@@ -1,8 +1,133 @@
-Require Import String.
+(*The examples here are taken from the semantics course material on the separation 
+  logic framework Iris, available at
+  https://plv.mpi-sws.org/semantics-course/
+*)
 
+Require Import String.
 Inductive expr :=
   | Var (x : string)
   | Lam (x : string) (e : expr)
   | App (e1 e2 : expr)
   | LitInt (n: nat)
   | Plus (e1 e2 : expr).
+
+Declare Scope expr_scope.
+Declare Scope val_scope.
+Delimit Scope expr_scope with E.
+Delimit Scope val_scope with V.
+
+Definition is_val (e: expr): Prop := 
+  match e with
+  | LitInt n => True
+  | Lam x e => True
+  | _ => False
+  end.
+
+Inductive val :=
+  | LitIntV (n: nat)
+  | LamV (x : string) (e : expr).
+
+
+(* Turn values into expressions*)
+Definition of_val (v : val) : expr :=
+  match v with
+  | LitIntV n => LitInt n
+  | LamV x e => Lam x e
+  end.
+
+(* try to turn expressions into values *)
+Definition to_val (e : expr) : option val :=
+  match e with
+  | LitInt n => Some (LitIntV n)
+  | Lam x e => Some (LamV x e)
+  | _ => None
+  end.
+
+Lemma to_of_val v : to_val (of_val v) = Some v.
+Proof.
+  destruct v; simpl; reflexivity.
+Qed.
+
+Lemma of_to_val e v : to_val e = Some v -> of_val v = e.
+Proof.
+  destruct e; simpl; try congruence.
+  all: injection 1 as <-; simpl; reflexivity.
+Qed.
+
+
+
+(** *** Substitution *)
+Fixpoint subst (x : string) (es : expr) (e : expr)  : expr :=
+  match e with
+  | LitInt n => LitInt n
+  | Var y => if (eqb x y) then es else Var y
+  | Lam y e =>
+      Lam y (if (eqb x y) then e else subst x es e)
+  | App e1 e2 => App (subst x es e1) (subst x es e2)
+  | Plus e1 e2 => Plus (subst x es e1) (subst x es e2)
+  end.
+
+
+(** *** Small-Step Semantics *)
+(* We use right-to-left evaluation order,
+   which means in a binary term (e.g., e1 + e2),
+   the left side can only be reduced once the right
+   side is fully evaluated (i.e., is a value). *)
+Inductive step : expr -> expr -> Prop :=
+  | StepBeta x e e'  :
+      is_val e' ->
+      step (App (Lam x e) e') (subst x e' e)
+  | StepAppL e1 e1' e2 :
+    is_val e2 ->
+    step e1 e1' ->
+    step (App e1 e2) (App e1' e2)
+  | StepAppR e1 e2 e2' :
+    step e2 e2' ->
+    step (App e1 e2) (App e1 e2')
+  | StepPlusRed (n1 n2 n3: nat) :
+    (n1 + n2)%nat = n3 ->
+    step (Plus (LitInt n1) (LitInt n2)) (LitInt n3)
+  | StepPlusL e1 e1' e2 :
+    is_val e2 ->
+    step e1 e1' ->
+    step (Plus e1 e2) (Plus e1' e2)
+  | StepPlusR e1 e2 e2' :
+    step e2 e2' ->
+    step (Plus e1 e2) (Plus e1 e2').
+
+(* We make the tactic eauto aware of the constructors of [step].
+   Then it can automatically solve goals where we want to prove a step. *)
+#[global] Hint Constructors step : core.
+
+
+(*Simple example of a user defined tactic.*)
+Ltac user_def_invert H :=
+  inversion H; subst; clear H.
+
+
+(*Examples for Scopes*)
+
+Inductive penguins : Set := 
+  | Penguinegg 
+  | Penguin
+  | Huddle (n: nat).
+
+Definition huddle (p1 p2: penguins) : penguins := 
+  match p1 with
+  | Huddle n => match p2 with 
+                 | Huddle m => Huddle (n + m)
+                 | _        => Huddle (S n)
+                end
+  | _        => Huddle (S (S 0))
+  end.
+
+Declare Scope penguins_scope.
+Delimit Scope penguins_scope with Peng.
+Declare Scope expr_scope.
+Delimit Scope expr_scope with E.
+
+Notation "p1 + p2" := (huddle p1 p2)
+                      (at level 50, left associativity)
+                       : penguins_scope.
+
+Notation "e1 + e2" := (Plus e1%E e2%E) : expr_scope.
